% Accompanying explanations and equations for replicating Kaplan & Violante 2010

%-------------------------------------
% CONFIGURATION
%-------------------------------------

\documentclass[11pt]{article}
\usepackage{amsmath}
\usepackage{amsfonts}

%-------------------------------------
% DOCUMENT
%-------------------------------------

\begin{document}

Omit i subscripts...

$$ u(c_t) = \frac{1}{1-\gamma} c^{1-\gamma} $$
$$ u_c(c_t) = c_t^{-\gamma} $$

\section*{Retirement (FOC for T$_{ret}$-1:T-2)}

Adapted from KV2010 ???:
\begin{equation*}
\begin{split}
 V_{t}(a_{t+1}, \tilde{y}) &= \max_{c_t,a_{t+1}} u(c_{t}) + \beta \mathbb{E}_t[V_{t+1}(a_{t+2}, \tilde{y})] \\
  \text{s.t. } c_t &= (1+r) a_{t}+P(\tilde{y}) - \frac{\xi_{t}}{\xi_{t+1}} a_{t+1}
\end{split}
\end{equation*}

$$ \frac{\partial{u(c_t)}}{\partial{a_{t+1}}} = -\frac{\xi_t}{\xi_{t+1}} c_t^{-\gamma} $$

$$ \frac{\partial{V_{t+1}(\cdot)}}{\partial{a_{t+1}}} = (1+r) c_{t+1}^{-\gamma} $$

$$ \Rightarrow c_t^{-\gamma} = \beta \frac{\xi_{t+1}}{\xi_t} (1+r) c_{t+1}^{-\gamma} $$
$$ \Rightarrow c_t = \left(\beta \frac{\xi_{t+1}}{\xi_t} (1+r) \right)^{-1/\gamma} c_{t+1} $$

FOC for retirement:
$$ \frac{\xi_t}{\xi_{t+1}} c_t^{-\gamma} = \beta \frac{\xi_t}{\xi_{t+1}} (1+r) c_{t+1}^{-\gamma} $$


Following Giovanni's notes, would have:
\begin{equation*}
\begin{split}
 V_{t}(a_{t+1}, \tilde{y}) &= \max_{c_t,a_{t+1}} u(c_{t}) + \beta \frac{\xi_{t+1}}{\xi_{t}} \mathbb{E}_t[V_{t+1}(a_{t+2}, \tilde{y})] \\
 \text{s.t. } c_t &= (1+r) a_{t}+P(\tilde{y}) - a_{t+1}
\end{split}
\end{equation*}

$$ \Rightarrow c_t^{-\gamma} = \beta \frac{\xi_{t+1}}{\xi_t} (1+r) c_{t+1}^{-\gamma} $$
$$ \Rightarrow c_t = \left(\beta \frac{\xi_{t+1}}{\xi_t} (1+r) \right)^{-1/\gamma} c_{t+1} $$


\section*{Working years (FOC for T=1:T$_{ret}$-2)}

\begin{equation*}
\begin{split}
 V_{t}(a_{t+1}, z_t) &= \max_{c_t,a_{t+1}} u(c_{t}) + \beta \mathbb{E}_t[V_{t+1}(a_{t+2}, z_{t+1})] \\
 \text{s.t. } c_t &= (1+r) a_{t}+y_t - a_{t+1}
\end{split}
\end{equation*}

$$ \Rightarrow c_t^{-\gamma} = \beta (1+r) \mathbb{E}_t [c_{t+1}^{-\gamma}] $$

\begin{equation*}
\begin{split}
\mathbb{E}_t [c_{t+1}^{-\gamma}] &=
      \mathbb{E}_t [\left( (1+r)a_{t+1} + y_{t+1} - a_{t+2} \right)^{-\gamma}] \\
      &= \mathbb{E}_t [\left((1+r)a_{t+1} + \exp(\kappa_{t+1} + z_{t+1} + \varepsilon_{t+1}) - a_{t+2} \right)^{-\gamma}] \\
      &= \sum_{z_{t+1}|z_t} \sum_{\varepsilon_t} \pi_{z,t}(z_{t+1}|z_t) \pi_\varepsilon(\varepsilon_{t+1}) \left((1+r)a_{t+1} + e^{(\kappa_{t+1} + z_{t+1} + \varepsilon_{t+1})} - a_{t+2} \right)^{-\gamma}
\end{split}
\end{equation*}


% \begin{equation*}
% \begin{aligned}
%    V_{t}\left(z_{t}, \eta_{t}\right)=& \max _{c_{t}, a_{t}} \log \left(c_{t}\right)+\beta \mathbb{E}_{t} V_{t+1}\left(z_{t+1}, \eta_{t+1}\right) \\
%    \text { s.t. } z_{t} &= (1+r) a_{t-1}+y_{t} \\
%    a_{t}+c_{t} &= z_{t} \\
%    \log y_{t} &= \eta_{t}+u_{t} \\
%    \eta_{t} &= \rho_{t} \eta_{t-1}+\varepsilon_{t} \\
%    \varepsilon_{t} &= P\left(0, \sigma_{\varepsilon t}\right), u_{t} \stackrel{i . i . d}{\sim} N\left(0, \sigma_{u}\right) \\
%     a_{t+1} \geq 0, & a_{0}, y_{0} \text { given. }
% \end{aligned}
% \end{equation*}


\end{document}


\\
&= \max_{a_t} u((1+r) a_{t}+P(\tilde{\mathbf{Y}}) - \frac{\xi_{t}}{\xi_{t+1}} a_{t+1}) + \beta \frac{\xi_{t+1}}{\xi_{t}} \mathbb{E}_t[\tilde{V}_{t+1}(a_{t+1}, c_{t+1}, z_{t+1})] \\
&= \sum_{z_{t+1}} \sum_{\varepsilon} \pi(z_{t+1}|z_t) \pi(\varepsilon)
 \tilde{V}_{t+1}(a_{t+1}, z_{t+1})

&= \sum_{\eta_{t+1}|z_t} \sum_{\varepsilon_t} \pi_{\eta,t}(\eta_{t+1}|z_t) \pi_\varepsilon(\varepsilon_{t+1}) \left((1+r)a_{t+1} + e^{(\kappa_{t+1} + z_t + \eta_{t+1} + \varepsilon_{t+1})} - a_{t+2} \right)^{-\gamma}
