%%%%%%%%%%%%%%%%%%%%%%%%%%%%%%%%%%%%%%
%
% General document
% LaTeX Template
%
% Author:
% Allen Peters
%
% Creation date:
% September 27, 2019
%
%%%%%%%%%%%%%%%%%%%%%%%%%%%%%%%%%%%%%%

%-------------------------------------
% CONFIGURATION
%-------------------------------------

\documentclass[11pt]{article}

\usepackage{geometry}
\geometry{
	paper=letterpaper, % Change to letterpaper for US letter
	top=2.5cm, % Top margin
	bottom=2.5cm, % Bottom margin
	left=2.5cm, % Left margin
	right=2.5cm, % Right margin
	%showframe, % Uncomment to show how the type block is set on the page
}

\usepackage[backend=biber,style=apa,autocite=inline]{biblatex} \DeclareLanguageMapping{english}{english-apa}
\addbibresource{/home/allenpeters/Data/Documents/PhD/EnviroMacro/enviroMacroBibDB.bib}

%\usepackage{stix} % Use the Stix font by default
%\usepackage{newtxtext,newtxmath} % closest to Times New Roman

\usepackage{microtype} % Improve justification

\usepackage{fancyhdr}
\pagestyle{fancy}
\fancyhf{}
\lhead{ECON 516/ECON 622}
\rhead{Allen Peters}
\cfoot{\thepage}

\author{}
\date{}
\title{}


%---------------------------------------
% DOCUMENT
%---------------------------------------

\begin{document}

\section*{Derivations for replication of Kaplan \& Violante (2010)}
This document contains derivations of Euler equations using the budget constraints in the paper, as well as a more standard version that does not scale assets by survival probability.

\subsection*{Functional forms employed}

\paragraph{Income process}
$$ y_{i t} =  \exp( \kappa_t + z_{i t} + \varepsilon_{i t})$$
$$ z_{i t} = z_{i,t-1} + \eta_{i t} $$

\paragraph{Utility Function}
(Omitting i subscripts)
$$ u(c_t) = \frac{1}{1-\gamma} c^{1-\gamma} $$
$$ u_c(c_t) = c_t^{-\gamma} $$


\subsection*{Standard budget constraint}

The following derivations are those implemented in the code {KV 2010.jl}. I omit $i$ subscripts.

\subsection*{Kaplan \& Violante's budget constraint}

The following derivations are following my interpretation of what is presented in the paper. I omit $i$ subscripts.

\paragraph{Budget constraints}
$$ c_t \frac{\xi_{t}}{\xi_{t+1}} a_{t+1} = (1+r) a_{t}+P(\tilde{y}) ~ $$
$$
\begin{aligned}
c_{t}+a_{t+1}=(1+r) a_{t}+y_{t}, \quad \text { if } t<T^{r e t}\\
&c_{t}+\left(\frac{\xi_{t}}{\xi_{t+1}}\right) a_{t+1}=(1+r) a_{t}+P\left(\tilde{\mathbf{Y}}_{i}\right), \quad \text { if } t \geq T^{r e t}
\end{aligned}
$$

\paragraph{Retirement (FOC for T$_{ret}$:T-1)}

\begin{equation*}
\begin{split}
 V_{t}(a_{t+1}, \tilde{y}) &= \max_{c_t,a_{t+1}} u(c_{t}) + \beta \frac{\xi_{t+1}}{\xi_{t}} \mathbb{E}_t[V_{t+1}(a_{t+2}, \tilde{y})] \\
  \text{s.t. } c_t &= (1+r) a_{t}+P(\tilde{y}) - \frac{\xi_{t}}{\xi_{t+1}} a_{t+1}
\end{split}
\end{equation*}

$$ \frac{\partial{u(c_t)}}{\partial{a_{t+1}}} = -\frac{\xi_t}{\xi_{t+1}} c_t^{-\gamma} $$

$$ \frac{\partial{V_{t+1}(\cdot)}}{\partial{a_{t+1}}} = (1+r) c_{t+1}^{-\gamma} $$

$$ \Rightarrow c_t^{-\gamma} = \beta \left(
    \frac{\xi_{t+1}}{\xi_t} \right) ^2 (1+r) c_{t+1}^{-\gamma} $$
$$ \Rightarrow c_t = \left(\beta \left(
    \frac{\xi_{t+1}}{\xi_t} \right) ^2 (1+r) \right)^{-1/\gamma} c_{t+1} $$

FOC for retirement:
$$ \frac{\xi_t}{\xi_{t+1}} c_t^{-\gamma} = \beta \frac{\xi_t}{\xi_{t+1}} (1+r) c_{t+1}^{-\gamma} $$


\paragraph{Following Giovanni's notes, would have:}
\begin{equation*}
\begin{split}
 V_{t}(a_{t+1}, \tilde{y}) &= \max_{c_t,a_{t+1}} u(c_{t}) + \beta \frac{\xi_{t+1}}{\xi_{t}} \mathbb{E}_t[V_{t+1}(a_{t+2}, \tilde{y})] \\
 \text{s.t. } c_t &= (1+r) a_{t}+P(\tilde{y}) - a_{t+1}
\end{split}
\end{equation*}

$$ \Rightarrow c_t^{-\gamma} = \beta \frac{\xi_{t+1}}{\xi_t} (1+r) c_{t+1}^{-\gamma} $$
$$ \Rightarrow c_t = \left(\beta \frac{\xi_{t+1}}{\xi_t} (1+r) \right)^{-1/\gamma} c_{t+1} $$


\paragraph{Working years (FOC for T=1:T$_{ret}$-2)}

\begin{equation*}
\begin{split}
 V_{t}(c_t + a_{t+1}, z_t) &= \max_{c_t,a_{t+1}} u(c_{t}) + \beta \mathbb{E}_t[V_{t+1}(c_{t+1} + a_{t+2}, z_{t+1})] \\
 \text{s.t. } c_t &= (1+r) a_{t}+y_t - a_{t+1}
\end{split}
\end{equation*}

$$ \Rightarrow c_t^{-\gamma} = \beta (1+r) \mathbb{E}_t [c_{t+1}^{-\gamma}] $$

\begin{equation}
\begin{split}
\mathbb{E}_t [c_{t+1}^{-\gamma}] &=
      \mathbb{E}_t [\left( (1+r)a_{t+1} + y_{t+1} - a_{t+2} \right)^{-\gamma}] \\
      &= \mathbb{E}_t [\left((1+r)a_{t+1} + \exp(\kappa_{t+1} + z_{t+1} + \varepsilon_{t+1}) - a_{t+2} \right)^{-\gamma}] \\
      &= \sum_{z_{t+1}|z_t} \sum_{\varepsilon_t} \pi_{z,t}(z_{t+1}|z_t) \pi_\varepsilon(\varepsilon_{t+1}) \left((1+r)a_{t+1} + e^{(\kappa_{t+1} + z_{t+1} + \varepsilon_{t+1})} - a_{t+2} \right)^{-\gamma}
\end{split}
\end{equation}

\begin{equation}
  \Rightarrow c_t = \left( \beta (1+r) \mathbb{E}_t [c_{t+1}^{-\gamma}]  \right) ^{-\frac{1}{\gamma}}
\end{equation}

\begin{equation}
\begin{split}
a_{t} &= \frac{1}{1+r} \left( c_t + a_{t+1} - y_t \right) \\
      &= \frac{1}{1+r} \left( c_t + a_{t+1} - \exp( \kappa_t + z_{t} + \varepsilon_{t}) \right)
\end{split}
\end{equation}


% \begin{equation*}
% \begin{aligned}
%    V_{t}\left(z_{t}, \eta_{t}\right)=& \max _{c_{t}, a_{t}} \log \left(c_{t}\right)+\beta \mathbb{E}_{t} V_{t+1}\left(z_{t+1}, \eta_{t+1}\right) \\
%    \text { s.t. } z_{t} &= (1+r) a_{t-1}+y_{t} \\
%    a_{t}+c_{t} &= z_{t} \\
%    \log y_{t} &= \eta_{t}+u_{t} \\
%    \eta_{t} &= \rho_{t} \eta_{t-1}+\varepsilon_{t} \\
%    \varepsilon_{t} &= P\left(0, \sigma_{\varepsilon t}\right), u_{t} \stackrel{i . i . d}{\sim} N\left(0, \sigma_{u}\right) \\
%     a_{t+1} \geq 0, & a_{0}, y_{0} \text { given. }
% \end{aligned}
% \end{equation*}


\end{document}


\\
&= \max_{a_t} u((1+r) a_{t}+P(\tilde{\mathbf{Y}}) - \frac{\xi_{t}}{\xi_{t+1}} a_{t+1}) + \beta \frac{\xi_{t+1}}{\xi_{t}} \mathbb{E}_t[\tilde{V}_{t+1}(a_{t+1}, c_{t+1}, z_{t+1})] \\
&= \sum_{z_{t+1}} \sum_{\varepsilon} \pi(z_{t+1}|z_t) \pi(\varepsilon)
 \tilde{V}_{t+1}(a_{t+1}, z_{t+1})

&= \sum_{\eta_{t+1}|z_t} \sum_{\varepsilon_t} \pi_{\eta,t}(\eta_{t+1}|z_t) \pi_\varepsilon(\varepsilon_{t+1}) \left((1+r)a_{t+1} + e^{(\kappa_{t+1} + z_t + \eta_{t+1} + \varepsilon_{t+1})} - a_{t+2} \right)^{-\gamma}


$$c_t + a_{t+1} &= (1+r) a_{t}+y_t = (1+r) a_{t} + \exp( \kappa_t + z_{t} + \varepsilon_{t})$$
